src/Init/Control/Traversable.lean
@@ -7,14 +7,13 @@ prelude
 import Init.Core
 
 /-
-  Typeclass for the polymorphic `foldlM` operation described in the paper.
+  Typeclass for the polymorphic `forM` operation described in the "do unchained" paper.
   Remark:
   - `γ` is a "container" type of elements of type `α`.
   - `α` is treated as an output parameter by the typeclass resolution procedure.
     That is, it tries to find an instance using only `m` and `γ`.
 -/
-class Foldable (m : Type u → Type v) (γ : Type w₁) (α : outParam (Type w₂)) where
-  foldlM [Monad m] : (δ → α → m δ) → δ → γ → m δ
+class Traversable (m : Type u → Type v) (γ : Type w₁) (α : outParam (Type w₂)) where
+  forM [Monad m] : γ → (α → m PUnit) → m PUnit
 
--- Add the alias `foldlM` for `Foldable.foldlM`
-export Foldable (foldlM)
+export Traversable (forM)
